\documentclass{article}
\usepackage{preamb/iris}
\usepackage{preamb/heaplang}
\usepackage{graphicx} % Required for inserting images
\usepackage{listings}
\usepackage{ebproof}
\usepackage{parskip}

\title{Program Logics Hand-in 1}
\author{Zijun Yu 202203581}
\date{September 2023}

\begin{document}
\include{preamb/macros.tex}

\maketitle

\section*{Exercise 1}

\subsection*{Part 1}

\begin{align*}
     & ([], [0 \mapsto \langkw{singleton} 1])                      \\
     & \cstepsto ([], [0 \mapsto \Inr (\Ref (1, \Inl ()))])        \\
     & \cstepsto ([l_1 \mapsto (1, \Inl())], [0 \mapsto \Inr l_1])
\end{align*}

\subsection*{Part 2}

\begin{align*}
     & ([], [0 \mapsto \langkw{inc} (\langkw{singleton} 1)])                                       \\
     & \cstepsto ([l_1 \mapsto (1, \Inl())], [0 \mapsto \langkw{inc} (\Inr l_1)])                  \\
     & \cstepsto ([l_1 \mapsto (1, \Inl())], [0 \mapsto                                            \\ & \quad
    \Match{\Inr l_1}with{\Inl x_1}=>{()}|{\Inr x_2}=>{
    \Let{v}={\pi_1(!x_2)}in \Let{t}={\pi_2(!x_2)}in{x_2 \leftarrow (v+1, t); \langkw{inc} t}
    }end])                                                                                         \\
     & \cstepsto ([l_1 \mapsto (1, \Inl())], [0 \mapsto
    \Let{v}={\pi_1(!l_1)}in \Let{t}={\pi_2(!l_1)}in{l_1 \leftarrow (v+1, t); \langkw{inc} t}])     \\
     & \cstepsto ([l_1 \mapsto (1, \Inl())], [0 \mapsto
    \Let{v}={\pi_1(1,\Inl())}in \Let{t}={\pi_2(!l_1)}in{l_1 \leftarrow (v+1, t); \langkw{inc} t}]) \\
     & \cstepsto ([l_1 \mapsto (1, \Inl())], [0 \mapsto
    \Let{v}={1}in \Let{t}={\pi_2(!l_1)}in{l_1 \leftarrow (v+1, t); \langkw{inc} t}])               \\
     & \cstepsto ([l_1 \mapsto (1, \Inl())], [0 \mapsto
    \Let{t}={\pi_2(!l_1)}in{l_1 \leftarrow (1+1, t); \langkw{inc} t}])                             \\
     & \cstepsto ([l_1 \mapsto (1, \Inl())], [0 \mapsto
    \Let{t}={\pi_2(1, \Inl())}in{l_1 \leftarrow (1+1, t); \langkw{inc} t}])                        \\
     & \cstepsto ([l_1 \mapsto (1, \Inl())], [0 \mapsto
    \Let{t}={\Inl()}in{l_1 \leftarrow (1+1, t); \langkw{inc} t}])                                  \\
     & \cstepsto ([l_1 \mapsto (1, \Inl())], [0 \mapsto
    l_1 \leftarrow (1+1, \langkw{\Inl()}); \langkw{inc} \ \Inl()])                                 \\
     & \cstepsto ([l_1 \mapsto (1, \Inl())], [0 \mapsto
    l_1 \leftarrow (2, \langkw{\Inl()}); \langkw{inc} \ \Inl()])                                   \\
     & \cstepsto ([l_1 \mapsto (2, \Inl())], [0 \mapsto
    (); \langkw{inc} \ \Inl()])                                                                    \\
     & \cstepsto ([l_1 \mapsto (2, \Inl())], [0 \mapsto
    \langkw{inc} \ \Inl()])                                                                        \\
     & \cstepsto ([l_1 \mapsto (2, \Inl())], [0 \mapsto                                            \\ & \quad
    \Match{\Inl()}with{\Inl x_1}=>{()}|{\Inr x_2}=>{
    \Let{v}={\pi_1(!x_2)}in \Let{t}={\pi_2(!x_2)}in{x_2 \leftarrow (v+1, t); \langkw{inc} t}
    }end])                                                                                         \\
     & \cstepsto ([l_1 \mapsto (2, \Inl())], [0 \mapsto ()])                                       \\
\end{align*}

The syntactic sugars are not expanded in the reduction.

\section*{Exercise 2}

\subsection*{Approach 1}

\begin{prooftree}
    \infer0{P \star Q \vdash P}
    \infer0{P \star Q \vdash Q}
    \infer2{P \star Q \vdash P \wedge Q}
\end{prooftree}

The usage of $\star-week$ and $\star-comm$ in proving $P\star Q \vdash Q$ is omitted.

\subsection*{Approach 2}

Using the result from Exercise 3:

\begin{prooftree}
    \infer0{P \wedge Q \vdash P \wedge Q}
    \infer1{P \vdash Q \wand (P \wedge Q)}
    \infer0{Q \vdash Q}
    \infer2{P \star Q \vdash P \wedge Q}
\end{prooftree}

\section*{Exercise 3}


\begin{prooftree}
    \hypo{P \vdash Q \wand R}
    \infer0{Q \vdash Q}
    \infer2{P \star Q \vdash R}
\end{prooftree}

\section*{Exercise 4}

From left to right:
\vspace{\baselineskip}

\begin{prooftree}
    \infer0{\Gamma \mid \exists x. P \star Q \vdash \exists x. P \star Q}
    \infer1{\Gamma, x \mid P \star Q \vdash \exists x. P \star Q}
    \infer1{\Gamma, x \mid Q \vdash P \wand \exists x. P \star Q}
    \infer1{\Gamma \mid \exists x. Q \vdash P \wand \exists x. P \star Q}
    \infer1{\Gamma \mid P \star \exists x . Q \vdash \exists x. P \star Q}
\end{prooftree}

\vspace{\baselineskip}
From right to left:
\vspace{\baselineskip}

\begin{prooftree}
    \infer0{\Gamma, x \mid P \vdash P}
    \infer0{\Gamma, x \mid \exists x. Q \vdash \exists x. Q}
    \infer1{\Gamma, x \mid Q \vdash \exists x. Q}
    \infer2{\Gamma, x \mid P \star Q \vdash P \star \exists x. Q}
    \infer1{\Gamma \mid \exists x. P \star Q \vdash P \star \exists x. Q}
\end{prooftree}

\end{document}